src/rocq/Semantics/Params/Address.v
@@ -14,6 +14,7 @@ From Stdlib Require Import OrderedType OrderedTypeEx.
 From Vellvm Require Import
   Utilities
   Params.Provenance.
+
 (* end hide *)
 
 (** * Signature for addresses
@@ -36,6 +37,18 @@ Class Address {P : Provenance} :=
     (* Debug *)
     show_addr : addr -> string;
   }.
+
+(* We pull this into a separate class to allow for a generic
+   implementation parametirized by any Address supporting PI.
+   Could be merged into Address if we don't care about that.
+ *)
+Class Overlaps {P : Provenance} {A : @Address P} :=
+  {
+      (** Do two memory regions overlap each other?
+        - *a1* and *a2* are addresses to the start of each region.
+        - *sz1* and *sz2* are the sizes of the two regions. *)
+    overlaps : addr -> Z -> addr -> Z -> bool ;
+}.
 
 (* TODO: Merge in the Address class, or keep it separate? *)
 (* TODO: Is it not over-engineering to allow margin for [ptr_to_int]
@@ -72,4 +85,47 @@ Class PITheory {P : Provenance} {A : @Address P} {P2I : @PI P A} :=
       int_to_ptr x p = ret a ->
       ptr_to_int a = x;
   }.
+
+From Vellvm Require Import
+  DynamicTypes
+  Params.Sizeof.
+Open Scope Z.
+
+Instance overlaps_ptoi {P : Provenance} {Ad : @Address P} {PI : @PI P Ad} :
+  @Overlaps P Ad :=
+  {|
+    overlaps (a1 : addr) (sz1 : Z) (a2 : addr) (sz2 : Z) :=
+      let a1_start := ptr_to_int a1 in
+      let a1_end   := ptr_to_int a1 + sz1 in
+      let a2_start := ptr_to_int a2 in
+      let a2_end   := ptr_to_int a2 + sz2 in
+      (a1_start <=? (a2_end - 1)) && (a2_start <=? (a1_end - 1))
+  |}.     
+
+(* TODO: Where should this kind of theory live?
+   It is awkward: it is generic to some extent, but depends on [dtyp].
+   Move simply on the Vellvm implementation side?
+   Move in the Params file?
+ *)
+Section Overlap.
+  Context {P : Provenance} {Ad : @Address P} {Si : Sizeof} {O : @Overlaps P Ad}.
+
+  (** Checks if two regions of memory overlap each other. The types
+   *τ1* and *τ2* are used to determine the size of the two memory
+        regions.
+   *)
+  Definition overlaps_dtyp (a1 : addr) (τ1 : dtyp) (a2 : addr) (τ2 : dtyp)
+    : bool :=
+    overlaps a1 (Z.of_N (sizeof_dtyp τ1)) a2 (Z.of_N (sizeof_dtyp τ2)).
+
+  (** Make sure that two regions of memory do not overlap *)
+  Definition no_overlap (a1 : addr) (sz1 : Z) (a2 : addr) (sz2 : Z) : bool
+    := negb (overlaps a1 sz1 a2 sz2).
+
+  (** Same as *no_overlap*, but using *dtyp*s *τ1* and *τ2* to
+        determine the size of the regions. *)
+  Definition no_overlap_dtyp (a1 : addr) (τ1 : dtyp) (a2 : addr) (τ2 : dtyp)
+    : bool := negb (overlaps_dtyp a1 τ1 a2 τ2).
+
+End Overlap.
 
